\documentclass[12pt]{article}
\usepackage{amsmath}

\setlength\parindent{0pt}
\renewcommand{\thesection}{\alph{section})}
\renewcommand{\thesubsection}{\thesection \arabic{subsection}}


\begin{document}

\section{}

$ \mathcal{X} = \{ A, B_1, B_2, C, D, E, F \} $ \\


$ \mathcal{A} = \{ a, b, c \} $ \\


$ \mathcal{Z} = \{ A, B, C, D, E, F \} $ \\

\section{}

$ P_a = \begin{bmatrix}
0   & 0.5 & 0.5 & 0   & 0   & 0   & 0 \\
0   & 0   & 0   & 0   & 0   & 1   & 0 \\
0   & 0   & 0   & 0   & 0   & 0   & 1 \\
0   & 1   & 0   & 0   & 0   & 0   & 0 \\
0   & 0   & 1   & 0   & 0   & 0   & 0 \\
1   & 0   & 0   & 0   & 0   & 0   & 0 \\
1   & 0   & 0   & 0   & 0   & 0   & 0 \\
\end{bmatrix} $

$ P_b = \begin{bmatrix}
0   & 0.5 & 0.5 & 0   & 0   & 0   & 0 \\
0   & 0   & 0   & 0   & 0   & 0   & 1 \\
0   & 0   & 0   & 0   & 0   & 1   & 0 \\
0   & 1   & 0   & 0   & 0   & 0   & 0 \\
0   & 0   & 1   & 0   & 0   & 0   & 0 \\
1   & 0   & 0   & 0   & 0   & 0   & 0 \\
1   & 0   & 0   & 0   & 0   & 0   & 0 \\
\end{bmatrix} $

$ P_c = \begin{bmatrix}
0   & 0.5 & 0.5 & 0   & 0   & 0   & 0 \\
0   & 0   & 0   & 1   & 0   & 0   & 0 \\
0   & 0   & 0   & 0   & 1   & 0   & 0 \\
0   & 1   & 0   & 0   & 0   & 0   & 0 \\
0   & 0   & 1   & 0   & 0   & 0   & 0 \\
1   & 0   & 0   & 0   & 0   & 0   & 0 \\
1   & 0   & 0   & 0   & 0   & 0   & 0 \\
\end{bmatrix} $

$ O_a = O_b = O_c = \begin{bmatrix}
1 & 0 & 0 & 0 & 0 & 0 \\
0 & 1 & 0 & 0 & 0 & 0 \\
0 & 1 & 0 & 0 & 0 & 0 \\
0 & 0 & 1 & 0 & 0 & 0 \\
0 & 0 & 0 & 1 & 0 & 0 \\
0 & 0 & 0 & 0 & 1 & 0 \\
0 & 0 & 0 & 0 & 0 & 1
\end{bmatrix}
$

$ c = \begin{bmatrix}
1 & 1 & 1 \\
1 & 1 & 1 \\
1 & 1 & 1 \\
1 & 1 & 1 \\
1 & 1 & 1 \\
1 & 1 & 1 \\
0 & 0 & 0 \\
\end{bmatrix}
$

\section{}
\subsection {}

$ b' = \frac{b_t P_a}{\Vert b_t P_a \Vert} $

$ b_t P_a = \begin{bmatrix}0 & .5 & .5 & 0 & 0 & 0 & 0\end{bmatrix} \times \begin{bmatrix}
0   & 0.5 & 0.5 & 0   & 0   & 0   & 0 \\
0   & 0   & 0   & 0   & 0   & 1   & 0 \\
0   & 0   & 0   & 0   & 0   & 0   & 1 \\
0   & 1   & 0   & 0   & 0   & 0   & 0 \\
0   & 0   & 1   & 0   & 0   & 0   & 0 \\
1   & 0   & 0   & 0   & 0   & 0   & 0 \\
1   & 0   & 0   & 0   & 0   & 0   & 0 \\
\end{bmatrix}$

$ = \begin{bmatrix}0 & 0 & 0 & 0 & 0 & .5 & .5\end{bmatrix} $

$\implies b' = \frac{\begin{bmatrix}0 & 0 & 0 & 0 & 0 & .5 & .5\end{bmatrix}}{\Vert\begin{bmatrix}0 & 0 & 0 & 0 & 0 & .5 & .5\end{bmatrix}\Vert} = \begin{bmatrix}0 & 0 & 0 & 0 & 0 & .5 & .5\end{bmatrix}$

\subsection{}

$ b' = \frac{b_t P_b}{\Vert b_t P_b \Vert} $

$ b_t P_a = \begin{bmatrix}0 & .5 & .5 & 0 & 0 & 0 & 0\end{bmatrix} \times \begin{bmatrix}
0   & 0.5 & 0.5 & 0   & 0   & 0   & 0 \\
0   & 0   & 0   & 0   & 0   & 0   & 1 \\
0   & 0   & 0   & 0   & 0   & 1   & 0 \\
0   & 1   & 0   & 0   & 0   & 0   & 0 \\
0   & 0   & 1   & 0   & 0   & 0   & 0 \\
1   & 0   & 0   & 0   & 0   & 0   & 0 \\
1   & 0   & 0   & 0   & 0   & 0   & 0 \\
\end{bmatrix}$

$ = \begin{bmatrix}0 & 0 & 0 & 0 & 0 & .5 & .5\end{bmatrix} $

$\implies b' = \frac{\begin{bmatrix}0 & 0 & 0 & 0 & 0 & .5 & .5\end{bmatrix}}{\Vert\begin{bmatrix}0 & 0 & 0 & 0 & 0 & .5 & .5\end{bmatrix}\Vert} = \begin{bmatrix}0 & 0 & 0 & 0 & 0 & .5 & .5\end{bmatrix} $

\subsection{}

$ b' = \frac{b_t P_c}{\Vert b_t P_c \Vert} $

$ b_t P_a = \begin{bmatrix}0 & .5 & .5 & 0 & 0 & 0 & 0\end{bmatrix} \times \begin{bmatrix}
0   & 0.5 & 0.5 & 0   & 0   & 0   & 0 \\
0   & 0   & 0   & 1   & 0   & 0   & 0 \\
0   & 0   & 0   & 0   & 1   & 0   & 0 \\
0   & 1   & 0   & 0   & 0   & 0   & 0 \\
0   & 0   & 1   & 0   & 0   & 0   & 0 \\
1   & 0   & 0   & 0   & 0   & 0   & 0 \\
1   & 0   & 0   & 0   & 0   & 0   & 0 \\
\end{bmatrix}$

$ = \begin{bmatrix}0 & 0 & 0 & .5 & .5 & 0 & 0 \end{bmatrix} $

$\implies b' = \frac{\begin{bmatrix}0 & 0 & 0 & .5 & .5 & 0 & 0 \end{bmatrix}}{\Vert\begin{bmatrix}0 & 0 & 0 & .5 & .5 & 0 & 0 \end{bmatrix}\Vert} = \begin{bmatrix}0 & 0 & 0 & .5 & .5 & 0 & 0 \end{bmatrix}$


\end{document}
